added half delta jump inversion

inversion/c/montgomery_jump_hd/template.c
@@ -1,0 +1,1 @@
+#include "../montgomery_jump_hd_template.c"
