src/Arithmetic/BYInv/Divstep.v
@@ -36,3 +36,27 @@ Fixpoint divstep_full_iter m d f g v r n :=
   | 0%nat => (d, f, g, v, r)
   | S n => let '(d, f, g, v, r) := divstep_full_iter m d f g v r n in divstep_spec_full m d f g v r
   end.
+
+Definition hddivstep_spec_full m d f g v r :=
+  if (0 <? d) && Z.odd g
+  then (2 - d, g, (g - f) / 2, 2 * r mod m, (r - v) mod m)
+  else (2 + d, f, (g + (g mod 2) * f) / 2, 2 * v mod m, (r + (g mod 2) * v) mod m).
+
+Definition hddivstep_spec_full' d f g u v q r :=
+  if (0 <? d) && Z.odd g
+  then (2 - d, g, (g - f) / 2,
+        2 * q, 2 * r, q - u, r - v)
+  else (2 + d, f, (g + (g mod 2) * f) / 2,
+        2 * u, 2 * v, q + (g mod 2) * u, r + (g mod 2) * v).
+
+Fixpoint hddivstep_spec_full'_iter d f g u v q r n :=
+  match n with
+  | 0%nat => (d, f, g, u, v, q, r)
+  | S n => let '(d, f, g, u, v, q, r) := hddivstep_spec_full'_iter d f g u v q r n in hddivstep_spec_full' d f g u v q r
+  end.
+
+Fixpoint hddivstep_full_iter m d f g v r n :=
+  match n with
+  | 0%nat => (d, f, g, v, r)
+  | S n => let '(d, f, g, v, r) := hddivstep_full_iter m d f g v r n in hddivstep_spec_full m d f g v r
+  end.
