src/Arithmetic/BYInv/BYInvJumpHd.v
@@ -1,0 +1,1447 @@
+Require Import Coq.ZArith.ZArith.
+Require Import Coq.Lists.List.
+Require Import Coq.micromega.Lia.
+
+Require Import Crypto.Arithmetic.UniformWeight.
+Require Import Crypto.Arithmetic.Saturated.
+Require Import Crypto.Arithmetic.Core.
+Require Import Crypto.Arithmetic.WordByWordMontgomery.
+
+Require Import Crypto.Arithmetic.BYInv.ArithmeticShiftr.
+Require Import Crypto.Arithmetic.BYInv.TCAdd.
+Require Import Crypto.Arithmetic.BYInv.EvalLemmas.
+Require Import Crypto.Arithmetic.BYInv.Divstep.
+Require Import Crypto.Arithmetic.BYInv.Definitions.
+Require Import Crypto.Arithmetic.BYInv.Ones.
+Require Import Crypto.Arithmetic.BYInv.TCSignExtend.
+Require Import Crypto.Arithmetic.BYInv.TCMul.
+Require Import Crypto.Arithmetic.BYInv.Firstn.
+
+Require Import Crypto.Util.LetIn.
+Require Import Crypto.Util.ListUtil.
+Require Import Crypto.Arithmetic.Partition.
+Require Import Crypto.Util.Decidable.
+Require Import Crypto.Util.ZUtil.Definitions.
+Require Import Crypto.Util.ZUtil.Modulo.
+Require Import Crypto.Util.ZUtil.Div.
+Require Import Crypto.Util.ZUtil.Odd.
+Require Import Crypto.Util.ZUtil.ArithmeticShiftr.
+Require Import Crypto.Util.ZUtil.Pow.
+Require Import Crypto.Util.ZUtil.TwosComplement.
+Require Import Crypto.Util.ZUtil.TwosComplementNeg.
+Require Import Crypto.Util.ZUtil.TwosComplementPos.
+Require Import Crypto.Util.ZUtil.TwosComplementOpp.
+Require Import Crypto.Arithmetic.ModOps.
+
+Require Import Crypto.Util.ZUtil.Tactics.PullPush.Modulo.
+
+Import Positional.
+Import ListNotations.
+Import Partition.
+
+Local Open Scope Z.
+Local Coercion Z.of_nat : nat >-> Z.
+Local Notation eval m n f := (Positional.eval (uweight m) n f).
+
+Hint Rewrite length_tc_add arithmetic_shiftr_length word_tc_mul_length : length_distr.
+
+(** Correctness of wordsized hddivstep *)
+Theorem twos_complement_word_full_hddivstep_correct
+        machine_wordsize d f g u v q r
+        (fodd : Z.odd f = true)
+        (mw1 : 2 < machine_wordsize)
+        (overflow_d : - 2 ^ (machine_wordsize - 1) + 2 <
+                      Z.twos_complement machine_wordsize d <
+                      2 ^ (machine_wordsize - 1) - 2)
+        (overflow_f : - 2 ^ (machine_wordsize - 2) <
+                      Z.twos_complement machine_wordsize f <
+                      2 ^ (machine_wordsize - 2))
+        (overflow_g : - 2 ^ (machine_wordsize - 2) <
+                      Z.twos_complement machine_wordsize g <
+                      2 ^ (machine_wordsize - 2))
+        (overflow_u : - 2 ^ (machine_wordsize - 2) <
+                      Z.twos_complement machine_wordsize u <
+                      2 ^ (machine_wordsize - 2))
+        (overflow_v : - 2 ^ (machine_wordsize - 2) <
+                      Z.twos_complement machine_wordsize v <
+                      2 ^ (machine_wordsize - 2))
+        (overflow_q : - 2 ^ (machine_wordsize - 2) <
+                      Z.twos_complement machine_wordsize q <
+                      2 ^ (machine_wordsize - 2))
+        (overflow_r : - 2 ^ (machine_wordsize - 2) <
+                      Z.twos_complement machine_wordsize r <
+                      2 ^ (machine_wordsize - 2))
+        (Hf2 : 0 <= f < 2^machine_wordsize)
+        (Hg2 : 0 <= g < 2^machine_wordsize) :
+  let '(d1,f1,g1,u1,v1,q1,r1) :=
+      (twos_complement_word_full_hddivstep machine_wordsize d f g u v q r) in
+  (Z.twos_complement machine_wordsize d1,
+   Z.twos_complement machine_wordsize f1,
+   Z.twos_complement machine_wordsize g1,
+   Z.twos_complement machine_wordsize u1,
+   Z.twos_complement machine_wordsize v1,
+   Z.twos_complement machine_wordsize q1,
+   Z.twos_complement machine_wordsize r1) =
+  hddivstep_spec_full' (Z.twos_complement machine_wordsize d)
+                     (Z.twos_complement machine_wordsize f)
+                     (Z.twos_complement machine_wordsize g)
+                     (Z.twos_complement machine_wordsize u)
+                     (Z.twos_complement machine_wordsize v)
+                     (Z.twos_complement machine_wordsize q)
+                     (Z.twos_complement machine_wordsize r).
+Proof.
+  assert (2 * 2 ^ (machine_wordsize - 2) = 2 ^ (machine_wordsize - 1)) by
+      (rewrite Z.pow_mul_base by lia; apply f_equal2; lia).
+  assert (2 ^ (machine_wordsize - 2) < 2^(machine_wordsize - 1)) by
+      (apply Z.pow_lt_mono_r; lia).
+  assert (2 <= 2 ^ (machine_wordsize - 2)) by
+      (replace 2 with (2 ^ 1) by lia; apply Z.pow_le_mono_r; lia).
+  unfold hddivstep_spec_full'; cbn -[Z.mul Z.add].
+  rewrite !Zselect.Z.zselect_correct.
+  rewrite !twos_complement_pos_spec, Zmod_odd, Z.twos_complement_odd by lia.
+  rewrite Z.twos_complement_mod2, (Zmod_odd g) by lia.
+  destruct (0 <? Z.twos_complement machine_wordsize d);
+    destruct (Z.odd g) eqn:godd;
+    rewrite (Zmod_odd); cbn -[Z.mul Z.add];
+      rewrite ?godd; cbn -[Z.mul Z.add].
+  rewrite <- (Z.twos_complement_odd machine_wordsize), !twos_complement_opp_spec by lia;
+    rewrite Z.odd_opp, Z.twos_complement_odd, fodd by lia; cbn -[Z.mul Z.add].
+  all: (repeat apply f_equal2;
+        repeat rewrite 1?Z.twos_complement_mod, 1?Z.twos_complement_add_full, 1?Z.twos_complement_one,
+        1?Z.arithmetic_shiftr1_spec, 1?twos_complement_opp_spec, 1?Z.twos_complement_zero;
+        rewrite ?Z.twos_complement_one, ?Z.twos_complement_two, ?twos_complement_opp_spec;
+        try apply Z.mod_pos_bound; try apply f_equal2; lia).
+Qed.
+
+Lemma twos_complement_word_full_hddivsteps_d_bound
+      machine_wordsize d f g u v q r n K
+      (Kpos : 0 <= K < 2 ^ (machine_wordsize - 1) - 2 * (Z.of_nat n))
+      (mw1 : 2 < machine_wordsize)
+      (overflow_d : - K <
+                    Z.twos_complement machine_wordsize d <
+                    K) :
+  let '(d1,_,_,_,_,_,_) :=
+      fold_left (fun data i => twos_complement_word_full_hddivstep_aux machine_wordsize data) (seq 0 n) (d,f,g,u,v,q,r) in
+  - K - 2 * Z.of_nat n <
+  Z.twos_complement machine_wordsize d1 <
+  K + 2 * Z.of_nat n.
+Proof.
+  induction n; intros.
+  - rewrite Z.add_0_r, Z.sub_0_r in *; cbn. assumption.
+  - rewrite seq_snoc, fold_left_app.
+    replace (Z.of_nat (S n)) with (1 + Z.of_nat n) in * by lia.
+    cbn -[Z.mul Z.add].
+    destruct (fold_left (fun (data : Z * Z * Z * Z * Z * Z * Z) (_ : nat)  => twos_complement_word_full_hddivstep_aux machine_wordsize data) _ _) as [[[[[[d1 f1] g1] u1] v1] q1] r1] eqn:E.
+    cbn -[Z.mul Z.add].
+
+    rewrite !Zselect.Z.zselect_correct, twos_complement_pos_spec, Zmod_odd by lia.
+    destruct (0 <? Z.twos_complement machine_wordsize d1);
+      destruct (Z.odd g1) eqn:g1odd; cbn -[Z.mul Z.add]; try assumption;
+        rewrite ?Z.twos_complement_mod, ?Z.twos_complement_add_full, ?twos_complement_opp_spec, ?Z.twos_complement_one, ?Z.twos_complement_two; try lia;
+          rewrite ?Z.twos_complement_mod, ?Z.twos_complement_add_full, ?twos_complement_opp_spec, ?Z.twos_complement_one, ?Z.twos_complement_two; try lia.
+Qed.
+
+Lemma twos_complement_word_full_hddivsteps_f_odd
+      machine_wordsize d f g u v q r n
+      (mw0 : 0 < machine_wordsize)
+      (fodd : Z.odd f = true) :
+  let '(_,f1,_,_,_,_,_) :=
+      fold_left (fun data i => twos_complement_word_full_hddivstep_aux machine_wordsize data) (seq 0 n) (d,f,g,u,v,q,r)  in
+  Z.odd f1 = true.
+Proof.
+  induction n; [assumption|].
+  rewrite seq_snoc, fold_left_app.
+  destruct (fold_left (fun (data : Z * Z * Z * Z * Z * Z * Z) (_ : nat)  => twos_complement_word_full_hddivstep_aux machine_wordsize data) _ _) as [[[[[[d1 f1] g1] u1] v1] q1] r1] eqn:E.
+  cbn -[Z.mul Z.add].
+  rewrite !Zselect.Z.zselect_correct.
+  destruct (dec _); [assumption|].
+  rewrite Zmod_odd in *. destruct (Z.odd g1). reflexivity. rewrite Z.land_0_r in n0. contradiction.
+Qed.
+
+Lemma div_lt_lower_bound a b c : 0 < b -> b * (a + 1) <= c -> a < c / b.
+Proof. intros; enough (a + 1 <= c / b) by lia; apply Z.div_le_lower_bound; assumption. Qed.
+
+Lemma twos_complement_word_full_hddivsteps_bounds
+      machine_wordsize d f g u v q r n K
+      (HK : 0 < K)
+      (HK2 : 2 ^ Z.of_nat n * K <= 2 ^ (machine_wordsize - 1))
+      (mw1 : 2 < machine_wordsize)
+      (fodd : Z.odd f = true)
+      (overflow_d : - (2 ^ (machine_wordsize - 1) - 1 - 2 * Z.of_nat n) <
+                    Z.twos_complement machine_wordsize d <
+                    2 ^ (machine_wordsize - 1) - 1 - 2 * Z.of_nat n)
+      (overflow_f : - 2 ^ (machine_wordsize - 2) <
+                    Z.twos_complement machine_wordsize f <
+                    2 ^ (machine_wordsize - 2))
+      (overflow_g : - 2 ^ (machine_wordsize - 2) <
+                    Z.twos_complement machine_wordsize g <
+                    2 ^ (machine_wordsize - 2))
+      (overflow_u : - K <
+                    Z.twos_complement machine_wordsize u <
+                    K)
+      (overflow_v : - K <
+                    Z.twos_complement machine_wordsize v <
+                    K)
+      (overflow_q : - K <
+                    Z.twos_complement machine_wordsize q <
+                    K)
+      (overflow_r : - K <
+                    Z.twos_complement machine_wordsize r <
+                    K) :
+  let '(_,f1,g1,u1,v1,q1,r1) :=
+      fold_left (fun data i => twos_complement_word_full_hddivstep_aux machine_wordsize data) (seq 0 n) (d,f,g,u,v,q,r) in
+      - 2 ^ (machine_wordsize - 2) <
+      Z.twos_complement machine_wordsize f1 <
+      2 ^ (machine_wordsize - 2) /\
+      - 2 ^ (machine_wordsize - 2) <
+      Z.twos_complement machine_wordsize g1 <
+      2 ^ (machine_wordsize - 2) /\
+      - 2 ^ n * K <
+      Z.twos_complement machine_wordsize u1 <
+      2 ^ n * K /\
+      - 2 ^ n * K <
+      Z.twos_complement machine_wordsize v1 <
+      2 ^ n * K /\
+      - 2 ^ n * K <
+      Z.twos_complement machine_wordsize q1 <
+      2 ^ n * K /\
+      - 2 ^ n * K <
+      Z.twos_complement machine_wordsize r1 <
+      2 ^ n * K.
+Proof.
+  assert (0 < 2 ^ machine_wordsize) by (apply Z.pow_pos_nonneg; lia).
+
+  induction n; intros.
+  - cbn -[Z.mul Z.add]; lia.
+  - replace (Z.of_nat (S n)) with (Z.of_nat n + 1) in * by lia.
+    rewrite <- Z.pow_mul_base in * by lia.
+
+    epose proof twos_complement_word_full_hddivsteps_d_bound _ _ f g u v q r n _ _ _ overflow_d.
+    epose proof twos_complement_word_full_hddivsteps_f_odd machine_wordsize d f g u v q r n _ _.
+
+    rewrite seq_snoc, fold_left_app.
+
+    cbn -[Z.mul Z.add].
+    destruct (fold_left (fun (data : Z * Z * Z * Z * Z * Z * Z) (_ : nat)  => twos_complement_word_full_hddivstep_aux machine_wordsize data) _ _) as [[[[[[d1 f1] g1] u1] v1] q1] r1] eqn:E.
+
+    specialize (IHn ltac:(lia) ltac:(lia)).
+    assert (2 * 2 ^ (machine_wordsize - 2) = 2 ^ (machine_wordsize - 1)) by
+        (rewrite Pow.Z.pow_mul_base; try apply f_equal2; lia).
+
+    cbn -[Z.mul Z.add].
+    rewrite !Zselect.Z.zselect_correct, twos_complement_pos_spec, Zmod_odd by lia.
+    destruct (0 <? Z.twos_complement machine_wordsize d1);
+      destruct (Z.odd g1) eqn:g1odd; cbn -[Z.mul Z.add].
+    + rewrite Zmod_odd, !twos_complement_opp_odd by (try assumption; lia). cbn -[Z.mul Z.add].
+      rewrite Z.arithmetic_shiftr1_spec by (try apply Z.mod_pos_bound; lia).
+      rewrite !Z.twos_complement_mod, !Z.twos_complement_add_full, !twos_complement_opp_spec by (try rewrite twos_complement_opp_spec; lia).
+      assert (forall a b, a <= b -> a / 2 <= b / 2) by (intros; apply Z.div_le_mono; lia).
+      repeat split; try apply div_lt_lower_bound; try apply Z.div_lt_upper_bound; lia.
+    + rewrite Zmod_odd, g1odd; cbn -[Z.mul Z.add]; rewrite !Z.add_0_r.
+      rewrite Z.arithmetic_shiftr1_spec by (try apply Z.mod_pos_bound; lia).
+      rewrite !Z.twos_complement_mod, !Z.twos_complement_add_full by lia.
+      repeat split; try apply div_lt_lower_bound; try apply Z.div_lt_upper_bound; lia.
+    + rewrite Zmod_odd, g1odd; cbn -[Z.mul Z.add].
+      rewrite Z.arithmetic_shiftr1_spec by (try apply Z.mod_pos_bound; lia).
+      rewrite !Z.twos_complement_mod, !Z.twos_complement_add_full by lia.
+      repeat split; try apply div_lt_lower_bound; try apply Z.div_lt_upper_bound; lia.
+    + rewrite Zmod_odd, g1odd; cbn -[Z.mul Z.add]; rewrite !Z.add_0_r.
+      rewrite Z.arithmetic_shiftr1_spec by (try apply Z.mod_pos_bound; lia).
+      rewrite !Z.twos_complement_mod, !Z.twos_complement_add_full by lia.
+      repeat split; try apply div_lt_lower_bound; try apply Z.div_lt_upper_bound; lia.
+
+      Unshelve. all: lia || assumption.
+Qed.
+
+Lemma twos_complement_word_full_hddivsteps_partial_bounds
+      machine_wordsize d f g u v q r n K
+      (HK : 0 < K)
+      (HK2 : 2 ^ Z.of_nat n * K <= 2 ^ (machine_wordsize - 1))
+      (mw1 : 2 < machine_wordsize)
+      (fodd : Z.odd f = true)
+      (u_pos : 0 <= u < 2 ^ machine_wordsize)
+      (v_pos : 0 <= v < 2 ^ machine_wordsize)
+      (q_pos : 0 <= q < 2 ^ machine_wordsize)
+      (r_pos : 0 <= r < 2 ^ machine_wordsize)
+      (overflow_d : - (2 ^ (machine_wordsize - 1) - 1 - 2 * Z.of_nat n) <
+                    Z.twos_complement machine_wordsize d <
+                    2 ^ (machine_wordsize - 1) - 1 - 2 * Z.of_nat n)
+      (overflow_u : - K <
+                    Z.twos_complement machine_wordsize u <
+                    K)
+      (overflow_v : - K <
+                    Z.twos_complement machine_wordsize v <
+                    K)
+      (overflow_q : - K <
+                    Z.twos_complement machine_wordsize q <
+                    K)
+      (overflow_r : - K <
+                    Z.twos_complement machine_wordsize r <
+                    K) :
+  let '(_,_,_,u1,v1,q1,r1) :=
+      fold_left (fun data i => twos_complement_word_full_hddivstep_aux machine_wordsize data) (seq 0 n) (d,f,g,u,v,q,r) in
+      - 2 ^ n * K <
+      Z.twos_complement machine_wordsize u1 <
+      2 ^ n * K /\
+      - 2 ^ n * K <
+      Z.twos_complement machine_wordsize v1 <
+      2 ^ n * K /\
+      - 2 ^ n * K <
+      Z.twos_complement machine_wordsize q1 <
+      2 ^ n * K /\
+      - 2 ^ n * K <
+      Z.twos_complement machine_wordsize r1 <
+      2 ^ n * K /\
+      0 <= u1 < 2 ^ machine_wordsize /\
+      0 <= v1 < 2 ^ machine_wordsize /\
+      0 <= q1 < 2 ^ machine_wordsize /\
+      0 <= r1 < 2 ^ machine_wordsize.
+Proof.
+  assert (0 < 2 ^ machine_wordsize) by (apply Z.pow_pos_nonneg; lia).
+
+  induction n; intros.
+  - cbn -[Z.mul Z.add]; lia.
+  - replace (Z.of_nat (S n)) with (Z.of_nat n + 1) in * by lia.
+    rewrite <- Z.pow_mul_base in * by lia.
+
+    epose proof twos_complement_word_full_hddivsteps_d_bound _ _ f g u v q r n _ _ _ overflow_d.
+    epose proof twos_complement_word_full_hddivsteps_f_odd machine_wordsize d f g u v q r n _ _.
+
+    rewrite seq_snoc, fold_left_app.
+
+    cbn -[Z.mul Z.add].
+    destruct (fold_left (fun (data : Z * Z * Z * Z * Z * Z * Z) (_ : nat)  => twos_complement_word_full_hddivstep_aux machine_wordsize data) _ _) as [[[[[[d1 f1] g1] u1] v1] q1] r1] eqn:E.
+
+    specialize (IHn ltac:(lia) ltac:(lia)).
+    assert (2 * 2 ^ (machine_wordsize - 2) = 2 ^ (machine_wordsize - 1)) by
+        (rewrite Pow.Z.pow_mul_base; try apply f_equal2; lia).
+
+    cbn -[Z.mul Z.add].
+    rewrite !Zselect.Z.zselect_correct, twos_complement_pos_spec, Zmod_odd by lia.
+    destruct (0 <? Z.twos_complement machine_wordsize d1);
+      destruct (Z.odd g1) eqn:g1odd; cbn -[Z.mul Z.add].
+    + rewrite Zmod_odd.
+      rewrite !twos_complement_opp_odd by (try assumption; lia).  cbn -[Z.mul Z.add].
+      rewrite !Z.twos_complement_mod, !Z.twos_complement_add_full, !twos_complement_opp_spec by (try rewrite twos_complement_opp_spec; lia).
+      assert (forall a b, a <= b -> a / 2 <= b / 2) by (intros; apply Z.div_le_mono; lia).
+      repeat split; try apply div_lt_lower_bound; try apply Z.div_lt_upper_bound; try apply Z.mod_pos_bound; try lia.
+    + rewrite Zmod_odd, g1odd; cbn -[Z.mul Z.add]; rewrite !Z.add_0_r.
+      rewrite !Z.twos_complement_mod, !Z.twos_complement_add_full by lia.
+      repeat split; try apply div_lt_lower_bound; try apply Z.div_lt_upper_bound; try apply Z.mod_pos_bound; lia.
+    + rewrite Zmod_odd, g1odd; cbn -[Z.mul Z.add].
+      rewrite !Z.twos_complement_mod, !Z.twos_complement_add_full by lia.
+      repeat split; try apply div_lt_lower_bound; try apply Z.div_lt_upper_bound; try apply Z.mod_pos_bound; lia.
+    + rewrite Zmod_odd, g1odd; cbn -[Z.mul Z.add]; rewrite !Z.add_0_r.
+      rewrite !Z.twos_complement_mod, !Z.twos_complement_add_full by lia.
+      repeat split; try apply div_lt_lower_bound; try apply Z.div_lt_upper_bound; try apply Z.mod_pos_bound; lia.
+
+      Unshelve. all: lia || assumption.
+Qed.
+
+Lemma twos_complement_word_full_hddivsteps_partial_bounds2
+      machine_wordsize d f g u v q r n K
+      (HK : 0 < K)
+      (HK2 : 2 ^ Z.of_nat n * K <= 2 ^ (machine_wordsize - 1))
+      (mw1 : 2 < machine_wordsize)
+      (fodd : Z.odd f = true)
+      (overflow_d : - (2 ^ (machine_wordsize - 1) - 1 - 2 * Z.of_nat n) <
+                    Z.twos_complement machine_wordsize d <
+                    2 ^ (machine_wordsize - 1) - 1 - 2 * Z.of_nat n)
+      (overflow_u : - K <
+                    Z.twos_complement machine_wordsize u <
+                    K)
+      (overflow_v : - K <
+                    Z.twos_complement machine_wordsize v <
+                    K)
+      (overflow_q : - K <
+                    Z.twos_complement machine_wordsize q <
+                    K)
+      (overflow_r : - K <
+                    Z.twos_complement machine_wordsize r <
+                    K) :
+  let '(_,_,_,u1,v1,q1,r1) :=
+      fold_left (fun data i => twos_complement_word_full_hddivstep_aux machine_wordsize data) (seq 0 n) (d,f,g,u,v,q,r) in
+      - 2 ^ n * K <
+      Z.twos_complement machine_wordsize u1 <
+      2 ^ n * K /\
+      - 2 ^ n * K <
+      Z.twos_complement machine_wordsize v1 <
+      2 ^ n * K /\
+      - 2 ^ n * K <
+      Z.twos_complement machine_wordsize q1 <
+      2 ^ n * K /\
+      - 2 ^ n * K <
+      Z.twos_complement machine_wordsize r1 <
+      2 ^ n * K.
+Proof.
+  assert (0 < 2 ^ machine_wordsize) by (apply Z.pow_pos_nonneg; lia).
+
+  induction n; intros.
+  - cbn -[Z.mul Z.add]; lia.
+  - replace (Z.of_nat (S n)) with (Z.of_nat n + 1) in * by lia.
+    rewrite <- Z.pow_mul_base in * by lia.
+
+    epose proof twos_complement_word_full_hddivsteps_d_bound _ _ f g u v q r n _ _ _ overflow_d.
+    epose proof twos_complement_word_full_hddivsteps_f_odd machine_wordsize d f g u v q r n _ _.
+
+    rewrite seq_snoc, fold_left_app.
+
+    cbn -[Z.mul Z.add].
+    destruct (fold_left (fun (data : Z * Z * Z * Z * Z * Z * Z) (_ : nat)  => twos_complement_word_full_hddivstep_aux machine_wordsize data) _ _) as [[[[[[d1 f1] g1] u1] v1] q1] r1] eqn:E.
+
+    specialize (IHn ltac:(lia) ltac:(lia)).
+    assert (2 * 2 ^ (machine_wordsize - 2) = 2 ^ (machine_wordsize - 1)) by
+        (rewrite Pow.Z.pow_mul_base; try apply f_equal2; lia).
+
+    cbn -[Z.mul Z.add].
+    rewrite !Zselect.Z.zselect_correct, twos_complement_pos_spec, Zmod_odd by lia.
+    destruct (0 <? Z.twos_complement machine_wordsize d1);
+      destruct (Z.odd g1) eqn:g1odd; cbn -[Z.mul Z.add].
+    + rewrite Zmod_odd,!twos_complement_opp_odd by (try assumption; lia). cbn -[Z.mul Z.add].
+      rewrite !Z.twos_complement_mod, !Z.twos_complement_add_full, !twos_complement_opp_spec
+        by (try rewrite twos_complement_opp_spec; lia).
+      assert (forall a b, a <= b -> a / 2 <= b / 2) by (intros; apply Z.div_le_mono; lia).
+      repeat split; try apply div_lt_lower_bound; try apply Z.div_lt_upper_bound; lia.
+    + rewrite Zmod_odd, g1odd; cbn -[Z.mul Z.add]; rewrite !Z.add_0_r.
+      rewrite !Z.twos_complement_mod, !Z.twos_complement_add_full by lia.
+      repeat split; try apply div_lt_lower_bound; try apply Z.div_lt_upper_bound; lia.
+    + rewrite Zmod_odd, g1odd; cbn -[Z.mul Z.add].
+      rewrite !Z.twos_complement_mod, !Z.twos_complement_add_full by lia.
+      repeat split; try apply div_lt_lower_bound; try apply Z.div_lt_upper_bound; lia.
+    + rewrite Zmod_odd, g1odd; cbn -[Z.mul Z.add]; rewrite !Z.add_0_r.
+      rewrite !Z.twos_complement_mod, !Z.twos_complement_add_full by lia.
+      repeat split; try apply div_lt_lower_bound; try apply Z.div_lt_upper_bound; lia.
+      Unshelve. all: lia || assumption. Qed.
+
+Theorem twos_complement_word_full_hddivstep_iter_correct
+        machine_wordsize d f g u v q r n K
+        (fodd : Z.odd f = true)
+        (HK : 2 ^ Z.of_nat n * K <= 2 ^ (machine_wordsize - 1))
+        (mw1 : 2 < machine_wordsize)
+        (overflow_d : - (2 ^ (machine_wordsize - 1) - 1 - 2 * Z.of_nat n) <
+                      Z.twos_complement machine_wordsize d <
+                      2 ^ (machine_wordsize - 1) - 1 - 2 * Z.of_nat n)
+        (overflow_f : - 2 ^ (machine_wordsize - 2) <
+                      Z.twos_complement machine_wordsize f <
+                      2 ^ (machine_wordsize - 2))
+        (overflow_g : - 2 ^ (machine_wordsize - 2) <
+                      Z.twos_complement machine_wordsize g <
+                      2 ^ (machine_wordsize - 2))
+        (overflow_u : - K <
+                      Z.twos_complement machine_wordsize u <
+                      K)
+        (overflow_v : - K <
+                      Z.twos_complement machine_wordsize v <
+                      K)
+        (overflow_q : - K <
+                      Z.twos_complement machine_wordsize q <
+                      K)
+        (overflow_r : - K <
+                      Z.twos_complement machine_wordsize r <
+                      K)
+        (Hf2 : 0 <= f < 2^machine_wordsize)
+        (Hg2 : 0 <= g < 2^machine_wordsize) :
+  let '(d1,f1,g1,u1,v1,q1,r1) :=
+      fold_left (fun data i => twos_complement_word_full_hddivstep_aux machine_wordsize data) (seq 0 n) (d,f,g,u,v,q,r)  in
+  (Z.twos_complement machine_wordsize d1,
+   Z.twos_complement machine_wordsize f1,
+   Z.twos_complement machine_wordsize g1,
+   Z.twos_complement machine_wordsize u1,
+   Z.twos_complement machine_wordsize v1,
+   Z.twos_complement machine_wordsize q1,
+   Z.twos_complement machine_wordsize r1) =
+  hddivstep_spec_full'_iter (Z.twos_complement machine_wordsize d)
+                          (Z.twos_complement machine_wordsize f)
+                          (Z.twos_complement machine_wordsize g)
+                          (Z.twos_complement machine_wordsize u)
+                          (Z.twos_complement machine_wordsize v)
+                          (Z.twos_complement machine_wordsize q)
+                          (Z.twos_complement machine_wordsize r) n.
+Proof.
+  assert (0 < 2 ^ machine_wordsize) by (apply Z.pow_pos_nonneg; lia).
+  assert (2 * 2 ^ (machine_wordsize - 2) = 2 ^ (machine_wordsize - 1)) by
+      (rewrite Pow.Z.pow_mul_base; try apply f_equal2; lia).
+
+  induction n; intros.
+  - reflexivity.
+  - replace (Z.of_nat (S n)) with (Z.of_nat n + 1) in * by lia.
+    rewrite <- Z.pow_mul_base in * by lia.
+
+    epose proof twos_complement_word_full_hddivsteps_d_bound _ _ f g u v q r n _ _ _ overflow_d.
+    epose proof twos_complement_word_full_hddivsteps_f_odd machine_wordsize d f g u v q r n _ _.
+    epose proof twos_complement_word_full_hddivsteps_bounds machine_wordsize d f g u v q r n K _ _ _ _ _ _ _ _ _ _ _.
+
+    rewrite seq_snoc, fold_left_app. cbn -[Z.mul Z.add].
+    destruct (fold_left (fun (data : Z * Z * Z * Z * Z * Z * Z) (_ : nat)  => twos_complement_word_full_hddivstep_aux machine_wordsize data) _ _) as [[[[[[d1 f1] g1] u1] v1] q1] r1] eqn:E.
+    rewrite <- IHn by lia.
+    cbn -[Z.mul Z.add].
+    unfold hddivstep_spec_full'.
+    rewrite !Zselect.Z.zselect_correct, Z.twos_complement_odd, twos_complement_pos_spec, Zmod_odd by lia.
+
+    destruct (0 <? Z.twos_complement machine_wordsize d1);
+      destruct (Z.odd g1) eqn:g1odd; cbn -[Z.mul Z.add].
+    + rewrite Zmod_odd, twos_complement_opp_odd by (try assumption; lia). cbn -[Z.mul Z.add].
+      repeat apply f_equal2; try reflexivity.
+      * rewrite Z.twos_complement_mod, Z.twos_complement_add_full, twos_complement_opp_spec, Z.twos_complement_two;
+          try rewrite ?twos_complement_opp_spec, ?Z.twos_complement_two; lia.
+      * rewrite Z.arithmetic_shiftr1_spec by (try apply Z.mod_pos_bound; lia).
+        rewrite Z.twos_complement_mod by lia.
+        rewrite Z.twos_complement_add_full by (try rewrite twos_complement_opp_spec; lia).
+        rewrite twos_complement_opp_spec by lia. apply f_equal2; lia.
+      * rewrite Z.twos_complement_mod, Z.twos_complement_add_full; lia.
+      * rewrite Z.twos_complement_mod, Z.twos_complement_add_full; lia.
+      * rewrite Z.twos_complement_mod, Z.twos_complement_add_full; try rewrite twos_complement_opp_spec; lia.
+      * rewrite Z.twos_complement_mod, Z.twos_complement_add_full; try rewrite twos_complement_opp_spec; lia.
+    + rewrite !Zmod_odd, Z.twos_complement_odd, g1odd, !Z.mul_0_l, !Z.add_0_r by lia; cbn -[Z.mul Z.add].
+      repeat match goal with
+             | [ |- (_, _) = (_, _) ] => apply f_equal2
+             end; try reflexivity.
+      * rewrite Z.twos_complement_mod, Z.twos_complement_add_full, Z.twos_complement_two;
+          try rewrite Z.twos_complement_two; lia.
+      * rewrite Z.arithmetic_shiftr1_spec, Z.twos_complement_mod; try apply Z.mod_pos_bound; lia.
+      * rewrite Z.twos_complement_mod, Z.twos_complement_add_full; lia.
+      * rewrite Z.twos_complement_mod, Z.twos_complement_add_full; lia.
+      * rewrite Z.twos_complement_mod; lia.
+      * rewrite Z.twos_complement_mod; lia.
+    + rewrite !Zmod_odd, Z.twos_complement_odd, g1odd, !Z.mul_1_l by lia; cbn -[Z.mul Z.add].
+      repeat match goal with
+             | [ |- (_, _) = (_, _) ] => apply f_equal2
+             end; try reflexivity.
+      * rewrite Z.twos_complement_mod, Z.twos_complement_add_full, Z.twos_complement_two; try rewrite Z.twos_complement_two; lia.
+      * rewrite Z.arithmetic_shiftr1_spec, Z.twos_complement_mod, Z.twos_complement_add_full; try apply Z.mod_pos_bound; lia.
+      * rewrite Z.twos_complement_mod, Z.twos_complement_add_full; lia.
+      * rewrite Z.twos_complement_mod, Z.twos_complement_add_full; lia.
+      * rewrite Z.twos_complement_mod, Z.twos_complement_add_full; lia.
+      * rewrite Z.twos_complement_mod, Z.twos_complement_add_full; lia.
+    + rewrite !Zmod_odd, Z.twos_complement_odd, g1odd, !Z.mul_0_l, !Z.add_0_r by lia; cbn -[Z.mul Z.add].
+      repeat match goal with
+             | [ |- (_, _) = (_, _) ] => apply f_equal2
+             end; try reflexivity.
+      * rewrite Z.twos_complement_mod, Z.twos_complement_add_full, Z.twos_complement_two; try rewrite Z.twos_complement_two; lia.
+      * rewrite Z.arithmetic_shiftr1_spec, Z.twos_complement_mod; try apply Z.mod_pos_bound; lia.
+      * rewrite Z.twos_complement_mod, Z.twos_complement_add_full; lia.
+      * rewrite Z.twos_complement_mod, Z.twos_complement_add_full; lia.
+      * rewrite Z.twos_complement_mod; lia.
+      * rewrite Z.twos_complement_mod; lia.
+
+        Unshelve. all: lia || assumption.
+Qed.
+
+Theorem twos_complement_word_full_hddivstep_iter_partially_correct
+        machine_wordsize d f g u v q r n K
+        (fodd : Z.odd f = true)
+        (HK : 2 ^ Z.of_nat n * K <= 2 ^ (machine_wordsize - 1))
+        (mw1 : 2 < machine_wordsize)
+        (nmw : n < machine_wordsize)
+        (overflow_d : - (2 ^ (machine_wordsize - 1) - 1 - 2 * Z.of_nat n) <
+                      Z.twos_complement machine_wordsize d <
+                      2 ^ (machine_wordsize - 1) - 1 - 2 * Z.of_nat n)
+        (overflow_u : - K <
+                      Z.twos_complement machine_wordsize u <
+                      K)
+        (overflow_v : - K <
+                      Z.twos_complement machine_wordsize v <
+                      K)
+        (overflow_q : - K <
+                      Z.twos_complement machine_wordsize q <
+                      K)
+        (overflow_r : - K <
+                      Z.twos_complement machine_wordsize r <
+                      K)
+        (u_pos : 0 <= u < 2 ^ machine_wordsize)
+        (v_pos : 0 <= v < 2 ^ machine_wordsize)
+        (q_pos : 0 <= q < 2 ^ machine_wordsize)
+        (r_pos : 0 <= r < 2 ^ machine_wordsize)
+        (Hf2 : 0 <= f < 2^machine_wordsize)
+        (Hg2 : 0 <= g < 2^machine_wordsize) :
+  let '(d1,f1,g1,u1,v1,q1,r1) :=
+      fold_left (fun data i => twos_complement_word_full_hddivstep_aux machine_wordsize data) (seq 0 n) (d,f,g,u,v,q,r)  in
+  (Z.twos_complement machine_wordsize d1,
+   Z.twos_complement machine_wordsize f1 mod 2 ^ (machine_wordsize - Z.of_nat n),
+   Z.twos_complement machine_wordsize g1 mod 2 ^ (machine_wordsize - Z.of_nat n),
+   Z.twos_complement machine_wordsize u1,
+   Z.twos_complement machine_wordsize v1,
+   Z.twos_complement machine_wordsize q1,
+   Z.twos_complement machine_wordsize r1) =
+  let '(d1',f1',g1',u1',v1',q1',r1') := hddivstep_spec_full'_iter (Z.twos_complement machine_wordsize d)
+                                                         (Z.twos_complement machine_wordsize f)
+                                                         (Z.twos_complement machine_wordsize g)
+                                                         (Z.twos_complement machine_wordsize u)
+                                                         (Z.twos_complement machine_wordsize v)
+                                                         (Z.twos_complement machine_wordsize q)
+                                                         (Z.twos_complement machine_wordsize r) n in
+  (d1', f1' mod 2 ^ (machine_wordsize - Z.of_nat n), g1' mod 2 ^ (machine_wordsize - Z.of_nat n), u1',v1',q1',r1').
+Proof.
+  assert (0 < 2 ^ machine_wordsize) by (apply Z.pow_pos_nonneg; lia).
+  assert (2 * 2 ^ (machine_wordsize - 2) = 2 ^ (machine_wordsize - 1)) by
+      (rewrite Pow.Z.pow_mul_base; try apply f_equal2; lia).
+
+  induction n.
+  - reflexivity.
+  - replace (Z.of_nat (S n)) with (Z.of_nat n + 1) in * by lia.
+    rewrite <- Z.pow_mul_base in * by lia.
+
+    epose proof twos_complement_word_full_hddivsteps_d_bound _ _ f g u v q r n _ _ _ overflow_d.
+    epose proof twos_complement_word_full_hddivsteps_f_odd machine_wordsize d f g u v q r n _ _.
+    epose proof twos_complement_word_full_hddivsteps_partial_bounds machine_wordsize d f g u v q r n K _ _ _ _ _ _ _ _ _.
+
+    rewrite seq_snoc, fold_left_app. cbn -[Z.mul Z.add].
+    destruct (fold_left (fun (data : Z * Z * Z * Z * Z * Z * Z) (_ : nat)  => twos_complement_word_full_hddivstep_aux machine_wordsize data) _ _) as [[[[[[d1 f1] g1] u1] v1] q1] r1] eqn:E1.
+    destruct (hddivstep_spec_full'_iter (Z.twos_complement machine_wordsize d) (Z.twos_complement machine_wordsize f)
+        (Z.twos_complement machine_wordsize g) (Z.twos_complement machine_wordsize u) (Z.twos_complement machine_wordsize v)
+        (Z.twos_complement machine_wordsize q) (Z.twos_complement machine_wordsize r) n) as [[[[[[d1' f1'] g1'] u1'] v1'] q1'] r1'] eqn:E2 .
+
+    assert ((Z.twos_complement machine_wordsize d1, Z.twos_complement machine_wordsize f1 mod 2 ^ (machine_wordsize - Z.of_nat n),
+        Z.twos_complement machine_wordsize g1 mod 2 ^ (machine_wordsize - Z.of_nat n), Z.twos_complement machine_wordsize u1,
+        Z.twos_complement machine_wordsize v1, Z.twos_complement machine_wordsize q1, Z.twos_complement machine_wordsize r1) =
+        (d1', f1' mod 2 ^ (machine_wordsize - Z.of_nat n), g1' mod 2 ^ (machine_wordsize - Z.of_nat n), u1', v1', q1', r1')).
+    apply IHn; lia.
+    inversion H4.
+
+    rewrite Z.twos_complement_mod_smaller_pow in H7 by lia.
+    rewrite Z.twos_complement_mod_smaller_pow in H8 by lia.
+
+    cbn -[Z.mul Z.add].
+    unfold hddivstep_spec_full'.
+    rewrite !Zselect.Z.zselect_correct, twos_complement_pos_spec, Zmod_odd by lia.
+
+    assert (Z.odd g1 = Z.odd g1').
+    { rewrite <- (Z.odd_mod2m (machine_wordsize - Z.of_nat n) g1'), <- H8, Z.odd_mod2m by lia; reflexivity. }
+    rewrite <- H5.
+    destruct (0 <? Z.twos_complement machine_wordsize d1);
+      destruct (Z.odd g1) eqn:g1odd; cbn -[Z.mul Z.add].
+    + rewrite Zmod_odd, twos_complement_opp_odd by (try assumption; lia).
+      cbn -[Z.mul Z.add].
+      repeat match goal with
+             | [ |- (_, _) = (_, _) ] => apply f_equal2
+             end.
+      * rewrite Z.twos_complement_mod, Z.twos_complement_add_full, twos_complement_opp_spec, Z.twos_complement_two by
+            (try rewrite twos_complement_opp_spec, Z.twos_complement_two; lia); lia.
+      *
+        rewrite Z.twos_complement_mod_smaller_pow, <- Z.mod_pow_same_base_smaller with (n:=(machine_wordsize - Z.of_nat n)) by lia.
+        rewrite H8, Z.mod_pow_same_base_smaller; lia.
+      * rewrite Z.arithmetic_shiftr1_spec, Z.twos_complement_mod by (try apply Z.mod_pos_bound; lia).
+        rewrite !Z.mod_pull_div by (apply Z.pow_nonneg; lia).
+        apply f_equal2; [|reflexivity].
+        replace (2 ^ (machine_wordsize - (Z.of_nat n + 1)) * 2) with (2 ^ (machine_wordsize - Z.of_nat n)) by
+            (rewrite Z.mul_comm, Z.pow_mul_base; [apply f_equal2|]; lia).
+        rewrite twos_complement_opp_correct, Z.twos_complement_mod_smaller_pow, <- Zplus_mod_idemp_l, Z.mod_pow_same_base_smaller, Zplus_mod_idemp_l by lia.
+        push_Zmod. rewrite H7, H8. pull_Zmod.
+        apply f_equal2; lia.
+      * rewrite Z.twos_complement_mod, Z.twos_complement_add_full; lia.
+      * rewrite Z.twos_complement_mod, Z.twos_complement_add_full; lia.
+      * rewrite Z.twos_complement_mod, Z.twos_complement_add_full,twos_complement_opp_spec; try rewrite twos_complement_opp_spec; lia.
+      * rewrite Z.twos_complement_mod, Z.twos_complement_add_full, twos_complement_opp_spec; try rewrite twos_complement_opp_spec; lia.
+    + rewrite !Zmod_odd, g1odd, <- H5, !Z.mul_0_l, !Z.add_0_r by lia; cbn -[Z.mul Z.add].
+      repeat match goal with
+             | [ |- (_, _) = (_, _) ] => apply f_equal2
+             end.
+      * rewrite Z.twos_complement_mod, Z.twos_complement_add_full, Z.twos_complement_two;
+          try rewrite Z.twos_complement_two; lia.
+      * rewrite Z.twos_complement_mod_smaller_pow, <- Z.mod_pow_same_base_smaller with (n:=(machine_wordsize - Z.of_nat n)), H7, Z.mod_pow_same_base_smaller; lia.
+      * rewrite Z.arithmetic_shiftr1_spec, Z.twos_complement_mod by (try apply Z.mod_pos_bound; lia).
+        rewrite !Z.mod_pull_div by (apply Z.pow_nonneg; lia).
+        apply f_equal2; [|reflexivity].
+        replace (2 ^ (machine_wordsize - (Z.of_nat n + 1)) * 2) with (2 ^ (machine_wordsize - Z.of_nat n)) by
+            (rewrite Z.mul_comm, Z.pow_mul_base; [apply f_equal2|]; lia).
+        rewrite Z.twos_complement_mod_smaller_pow; lia.
+      * rewrite Z.twos_complement_mod, Z.twos_complement_add_full; lia.
+      * rewrite Z.twos_complement_mod, Z.twos_complement_add_full; lia.
+      * rewrite Z.twos_complement_mod; lia.
+      * rewrite Z.twos_complement_mod; lia.
+    + rewrite !Zmod_odd, g1odd, <- H5, !Z.mul_1_l by lia; cbn -[Z.mul Z.add].
+      repeat match goal with
+             | [ |- (_, _) = (_, _) ] => apply f_equal2
+             end.
+      * rewrite Z.twos_complement_mod, Z.twos_complement_add_full, Z.twos_complement_two;
+          try rewrite Z.twos_complement_two; lia.
+      * rewrite Z.twos_complement_mod_smaller_pow, <- Z.mod_pow_same_base_smaller with (n:=(machine_wordsize - Z.of_nat n)), H7, Z.mod_pow_same_base_smaller; lia.
+      * rewrite Z.arithmetic_shiftr1_spec, Z.twos_complement_mod by (try apply Z.mod_pos_bound; lia).
+        rewrite !Z.mod_pull_div by (apply Z.pow_nonneg; lia).
+        apply f_equal2; [|reflexivity].
+        replace (2 ^ (machine_wordsize - (Z.of_nat n + 1)) * 2) with (2 ^ (machine_wordsize - Z.of_nat n)) by
+            (rewrite Z.mul_comm, Z.pow_mul_base; [apply f_equal2|]; lia).
+        rewrite Z.twos_complement_mod_smaller_pow by lia.
+        push_Zmod. rewrite H7, H8. pull_Zmod.
+        apply f_equal2; lia.
+      * rewrite Z.twos_complement_mod, Z.twos_complement_add_full; lia.
+      * rewrite Z.twos_complement_mod, Z.twos_complement_add_full; lia.
+      * rewrite Z.twos_complement_mod, Z.twos_complement_add_full; lia.
+      * rewrite Z.twos_complement_mod, Z.twos_complement_add_full; lia.
+    + rewrite !Zmod_odd, g1odd, <- H5, !Z.mul_0_l, !Z.add_0_r by lia; cbn -[Z.mul Z.add].
+      repeat match goal with
+             | [ |- (_, _) = (_, _) ] => apply f_equal2
+             end.
+      * rewrite Z.twos_complement_mod, Z.twos_complement_add_full, Z.twos_complement_two;
+          try rewrite Z.twos_complement_two; lia.
+      * rewrite Z.twos_complement_mod_smaller_pow, <- Z.mod_pow_same_base_smaller with (n:=(machine_wordsize - Z.of_nat n)), H7, Z.mod_pow_same_base_smaller; lia.
+      * rewrite Z.arithmetic_shiftr1_spec, Z.twos_complement_mod by (try apply Z.mod_pos_bound; lia).
+        rewrite !Z.mod_pull_div by (apply Z.pow_nonneg; lia).
+        apply f_equal2; [|reflexivity].
+        replace (2 ^ (machine_wordsize - (Z.of_nat n + 1)) * 2) with (2 ^ (machine_wordsize - Z.of_nat n)) by
+            (rewrite Z.mul_comm, Z.pow_mul_base; [apply f_equal2|]; lia).
+        rewrite Z.twos_complement_mod_smaller_pow; lia.
+      * rewrite Z.twos_complement_mod, Z.twos_complement_add_full; lia.
+      * rewrite Z.twos_complement_mod, Z.twos_complement_add_full; lia.
+      * rewrite Z.twos_complement_mod; lia.
+      * rewrite Z.twos_complement_mod; lia.
+
+      Unshelve.
+      all: try lia; try assumption.
+Qed.
+
+Lemma hddivstep_full_iter_full'_iter m d f g u2 v1 v2 q2 r1 r2 n :
+  let '(d1,f1,g1,_,_) :=
+      hddivstep_full_iter m d f g v1 r1 n in
+  (d1,f1,g1)
+  = let '(d2,f2,g2,_,_,_,_) := hddivstep_spec_full'_iter d f g u2 v2 q2 r2 n in
+    (d2,f2,g2).
+Proof.
+  induction n; simpl.
+  - reflexivity.
+  - destruct (hddivstep_full_iter m d f g v1 r1 n) as [[[[?]?]?]?].
+    destruct (hddivstep_spec_full'_iter d f g u2 v2 q2 r2 n) as [[[[[[?]?]?]?]?]?].
+    inversion IHn.
+    unfold hddivstep_spec_full'.
+    unfold hddivstep_spec_full.
+    destruct (0 <? z4); destruct (Z.odd z6); cbn -[Z.add Z.mul Z.div Z.sub]; reflexivity.
+Qed.
+
+Lemma hddivstep_full_iter_f_odd m f g v r n
+  (fodd : Z.odd f = true) :
+  let '(_,f,_,_,_) := hddivstep_full_iter m 1 f g v r n in Z.odd f = true.
+Proof.
+  induction n; simpl.
+  - assumption.
+  - unfold hddivstep_spec_full.
+    destruct (hddivstep_full_iter m 1 f g v r n) as [[[[d1 f1]g1]v1]r1].
+    destruct (0 <? d1); destruct (Z.odd g1) eqn:E; assumption.
+Qed.
+
+Lemma hddivstep_full'_iter_f_odd d f g u v q r n
+  (fodd : Z.odd f = true) :
+  let '(_,f,_,_,_,_,_) := hddivstep_spec_full'_iter d f g u v q r n in Z.odd f = true.
+Proof.
+  induction n; simpl.
+  - assumption.
+  - unfold hddivstep_spec_full'.
+    destruct (hddivstep_spec_full'_iter d f g u v q r n) as [[[[[[d1 f1]g1]u1]v1]q1]r1].
+    destruct (0 <? d1); destruct (Z.odd g1) eqn:E; assumption.
+Qed.
+
+Lemma hddivstep_full'_iter_important_bits d f f0 g g0 u v q r n k
+      (Hk : (0 <= n < k)%nat)
+      (fodd : Z.odd f = true)
+      (fmod : f mod 2 ^ Z.of_nat k = f0 mod 2 ^ Z.of_nat k)
+      (gmod : g mod 2 ^ Z.of_nat k = g0 mod 2 ^ Z.of_nat k) :
+  let '(d1,f1,g1,u1,v1,q1,r1) :=
+      hddivstep_spec_full'_iter d f g u v q r n in
+  let '(d2,f2,g2,u2,v2,q2,r2) :=
+      hddivstep_spec_full'_iter d f0 g0 u v q r n in
+  g1 mod 2 ^ (k - n) = g2 mod 2 ^ (k - n) /\
+  f1 mod 2 ^ (k - n) = f2 mod 2 ^ (k - n) /\
+  d1 = d2 /\
+  (u1,v1,q1,r1) = (u2,v2,q2,r2).
+Proof.
+  induction n.
+  - cbn in *. rewrite !Z.sub_0_r. repeat split; lia.
+  - simpl.
+
+    pose proof hddivstep_full'_iter_f_odd d f g u v q r n.
+    pose proof hddivstep_full'_iter_f_odd d f0 g0 u v q r n.
+
+    destruct (hddivstep_spec_full'_iter d f g u v q r n) as [[[[[[d1 f1] g1] u1] v1] q1] r1] eqn:E1.
+    destruct (hddivstep_spec_full'_iter d f0 g0 u v q r n) as [[[[[[d2 f2] g2] u2] v2] q2] r2] eqn:E2.
+
+    specialize (H fodd).
+    assert (Z.odd f0 = true).
+    { rewrite <- Z.odd_mod2m with (m:=k), <- fmod, Z.odd_mod2m; try assumption; lia. }
+
+    assert (g1 mod 2 ^ (Z.of_nat k - Z.of_nat n) = g2 mod 2 ^ (Z.of_nat k - Z.of_nat n) /\
+            f1 mod 2 ^ (Z.of_nat k - Z.of_nat n) = f2 mod 2 ^ (Z.of_nat k - Z.of_nat n) /\
+            d1 = d2 /\ (u1, v1, q1, r1) = (u2, v2, q2, r2)) by (apply IHn; lia).
+
+    destruct H2 as [H3 [H4 [H5 H6]]].
+
+    assert (Z.odd g1 = Z.odd g2 /\ d1 = d2).
+    { rewrite <- Z.odd_mod2m with (m:=k - n), H3, Z.odd_mod2m by lia; split; reflexivity || lia. }
+
+    unfold hddivstep_spec_full'. destruct H2. rewrite H7, H2.
+    inversion H6.
+
+    destruct (0 <? d2); destruct (Z.odd g2) eqn:odd; cbn -[Z.mul Z.add Z.div].
+    + split; [|split;[|split]]; try lia; try congruence.
+      * rewrite !Z.mod_pull_div, Z.mul_comm, Z.pow_mul_base by (try apply Z.pow_nonneg; lia).
+        replace (Z.of_nat k - Z.pos (Pos.of_succ_nat n) + 1) with (Z.of_nat k - Z.of_nat n) by lia.
+        push_Zmod. rewrite H3, H4. reflexivity.
+      * rewrite <- Z.mod_pow_same_base_smaller with (n:=(Z.of_nat k - Z.of_nat n)), H3, Z.mod_pow_same_base_smaller; lia.
+    + split; [|split;[|split]]; try reflexivity.
+      * rewrite !Z.mod_pull_div, (Z.mul_comm _ 2), Z.pow_mul_base by (try apply Z.pow_nonneg; lia).
+        replace (Z.of_nat k - Z.pos (Pos.of_succ_nat n) + 1) with (Z.of_nat k - Z.of_nat n) by lia.
+        push_Zmod. rewrite H3, H4, !Zmod_odd, odd, H2. reflexivity.
+      * rewrite <- Z.mod_pow_same_base_smaller with (n:=(Z.of_nat k - Z.of_nat n)), H4, Z.mod_pow_same_base_smaller; lia.
+      * rewrite !Zmod_odd, odd, H2; reflexivity.
+    + split; [|split;[|split]]; try reflexivity.
+      * rewrite !Z.mod_pull_div, (Z.mul_comm _ 2), Z.pow_mul_base by (try apply Z.pow_nonneg; lia).
+        replace (Z.of_nat k - Z.pos (Pos.of_succ_nat n) + 1) with (Z.of_nat k - Z.of_nat n) by lia.
+        push_Zmod. rewrite H3, H4, !Zmod_odd, odd, H2. reflexivity.
+      * rewrite <- Z.mod_pow_same_base_smaller with (n:=(Z.of_nat k - Z.of_nat n)), H4, Z.mod_pow_same_base_smaller; lia.
+      * rewrite !Zmod_odd, odd, H2; reflexivity.
+    + split; [|split;[|split]]; try reflexivity.
+      * rewrite !Z.mod_pull_div, (Z.mul_comm _ 2), Z.pow_mul_base by (try apply Z.pow_nonneg; lia).
+        replace (Z.of_nat k - Z.pos (Pos.of_succ_nat n) + 1) with (Z.of_nat k - Z.of_nat n) by lia.
+        push_Zmod. rewrite H3, H4, !Zmod_odd, odd, H2. reflexivity.
+      * rewrite <- Z.mod_pow_same_base_smaller with (n:=(Z.of_nat k - Z.of_nat n)), H4, Z.mod_pow_same_base_smaller; lia.
+      * rewrite !Zmod_odd, odd, H2; reflexivity.
+Qed.
+
+Lemma jump_hddivstep_full_iter m f g v r n
+      (fodd : Z.odd f = true)
+      (Hv : 0 <= v < m)
+      (Hr : 0 <= r < m)
+  :
+    let '(d1, f1, g1, v1, r1) := hddivstep_full_iter m 1 f g v r n in
+    (d1,2 ^ n * f1,2 ^ n * g1,v1,r1)
+  = let '(d1', f1', g1', u1', v1', q1', r1') := hddivstep_spec_full'_iter 1 f g 1 0 0 1 n in
+    (d1', (u1' * f + v1' * g), (q1' * f + r1' * g), (u1' * v + v1' * r) mod m, (q1' * v + r1' * r) mod m).
+Proof.
+  induction n.
+  - cbn -[Z.add Z.mul].
+    repeat match goal with
+           | [ |- (_, _) = (_, _) ] => apply f_equal2; rewrite ?Z.div_1_r, ?Z.mod_small by lia; try lia
+           end.
+  - cbn -[Z.pow Z.mul Z.add Z.of_nat].
+    pose proof hddivstep_full_iter_full'_iter m 1 f g 1 v 0 0 r 1 n.
+    pose proof hddivstep_full_iter_f_odd m f g v r n fodd as fodd1.
+
+    destruct (hddivstep_spec_full'_iter 1 f g 1 0 0 1 n) as [[[[[[d1 f1] g1] u1] v1] q1] r1] eqn:E1.
+    destruct (hddivstep_full_iter m 1 f g v r n) as [[[[d2 f2] g2] v2] r2] eqn:E2.
+
+    replace (Z.of_nat (S n)) with ((Z.of_nat n) + 1) by lia.
+    rewrite <- Z.pow_mul_base by lia.
+    unfold hddivstep_spec_full, hddivstep_spec_full'.
+    inversion H.
+    inversion IHn; subst.
+    destruct (0 <? d1); destruct (Z.odd g1) eqn:godd; cbn -[Z.mul Z.add Z.div Z.of_nat];
+      repeat match goal with
+             | [ |- (_, _) = (_, _) ] => apply f_equal2; try (push_Zmod; pull_Zmod; apply f_equal2; lia)
+             end; try lia.
+    rewrite <- Z.mul_assoc, Z.mul_comm, <- Z.mul_assoc, Z.mul_div_eq', Zmod_odd, Z.odd_sub, godd, fodd1; cbn; lia.
+    rewrite <- Z.mul_assoc, Z.mul_comm, <- Z.mul_assoc, Z.mul_div_eq', !Zmod_odd, godd, Z.add_0_r, godd; lia.
+    rewrite <- Z.mul_assoc, Z.mul_comm, <- Z.mul_assoc, Z.mul_div_eq', !Zmod_odd, godd, Z.mul_1_l, Z.odd_add, godd, fodd1, Z.sub_0_r; lia.
+    rewrite <- Z.mul_assoc, Z.mul_comm, <- Z.mul_assoc, Z.mul_div_eq', Zmod_odd, godd, Z.mul_0_l, Z.add_0_r, Zmod_odd, godd; lia.
+Qed.
+
+Lemma jump_hddivstep_full m f f0 g g0 v r n
+      (fodd : Z.odd f = true)
+      (Hm : 1 < m)
+      (Hv : 0 <= v < m)
+      (Hr : 0 <= r < m)
+      (Hf : f mod 2 ^ (Z.of_nat (S n)) = f0 mod 2 ^ (Z.of_nat (S n)))
+      (Hg : g mod 2 ^ (Z.of_nat (S n)) = g0 mod 2 ^ (Z.of_nat (S n)))
+  :
+  hddivstep_full_iter m 1 f g v r n
+  = let '(d1', f1', g1', u1', v1', q1', r1') := hddivstep_spec_full'_iter 1 f0 g0 1 0 0 1 n in
+    (d1', (u1' * f + v1' * g) / 2 ^ n, (q1' * f + r1' * g) / 2 ^ n, (u1' * v + v1' * r) mod m, (q1' * v + r1' * r) mod m).
+Proof.
+  assert (f0odd : Z.odd f0 = true).
+  { rewrite <- Z.odd_mod2m with (m:=S n), <- Hf, Z.odd_mod2m; try assumption; lia. }
+
+  pose proof jump_hddivstep_full_iter m f g v r n fodd Hv Hr.
+  pose proof hddivstep_full'_iter_important_bits 1 f f0 g g0 1 0 0 1 n (S n) ltac:(lia) fodd Hf Hg.
+
+  destruct (hddivstep_full_iter m 1 f g v r n) as [[[[d1 f1] g1] v1] r1] eqn:E1.
+  destruct (hddivstep_spec_full'_iter 1 f g 1 0 0 1 n) as [[[[[[d1' f1'] g1'] u1'] v1'] q1'] r1'] eqn:E2.
+  destruct (hddivstep_spec_full'_iter 1 f0 g0 1 0 0 1 n) as [[[[[[d1'' f1''] g1''] u1''] v1''] q1''] r1''] eqn:E3.
+  destruct H0 as [H1 [H2 [H3 H4]]].
+
+  inversion H; inversion H4; subst.
+
+  apply (f_equal (fun i => Z.div i (2 ^ Z.of_nat n))) in H6.
+  apply (f_equal (fun i => Z.div i (2 ^ Z.of_nat n))) in H7.
+  rewrite Z.div_mul' in * by (apply Z.pow_nonzero; lia).
+  congruence.
+Qed.
+
+(* TODO: Move thise *)
+Lemma fold_right_fold_left_lemma {A B : Type} (f : B -> A -> A) (l s : list B) (a : A) :
+  (forall x x' y, f x y = f x' y) -> length l = length s -> fold_left (fun i j => f j i) l a = fold_right f a s.
+Proof.
+  rewrite <- fold_left_rev_right. revert s a.
+  induction l; intros; simpl.
+  - assert (s = []) by (destruct s; simpl in *; try lia; reflexivity); subst. reflexivity.
+  - rewrite fold_right_snoc. replace s with (rev (rev s)) by (apply rev_involutive).
+    destruct (rev s) eqn:E.
+    apply (f_equal (@rev B)) in E. rewrite rev_involutive in E. subst. simpl in *. lia.
+    simpl. rewrite fold_right_snoc.
+    replace (f a a0) with (f b a0). apply IHl. assumption.
+    apply (f_equal (@length B)) in E. simpl in *.
+    rewrite rev_length in *. lia. apply H.
+Qed.
+
+Lemma pow_ineq k : (2 <= k)%nat -> k + 2 <= Zpower_nat 2 k.
+Proof. induction k as [|[|[|k]]]; [lia|lia|simpl; lia|rewrite Zpower_nat_succ_r; lia]; intros. Qed.
+
+Lemma pow_ineq_Z k : 2 <= k -> k + 2 <= 2 ^ k.
+Proof. intros. replace k with (Z.of_nat (Z.to_nat k)) by lia. rewrite <- Zpower_nat_Z. apply pow_ineq; lia. Qed.
+
+Lemma pow_ineq2 k : (3 <= k)%nat -> 2 * k + 2 <= Zpower_nat 2 k.
+Proof.
+  induction k; intros.
+  - lia.
+  - destruct k.
+    + lia.
+    + rewrite Zpower_nat_succ_r.
+      * destruct k.
+        ** simpl. lia.
+        ** destruct k.
+           *** simpl. lia.
+           *** lia.
+Qed.
+
+Lemma pow_ineq_Z2 k : 3 <= k -> 2 * k + 2 <= 2 ^ k.
+Proof.
+  intros. replace k with (Z.of_nat (Z.to_nat k)).
+  rewrite <- Zpower_nat_Z. apply pow_ineq2. lia. lia.
+Qed.
+
+Module WordByWordMontgomery.
+  Import WordByWordMontgomery.WordByWordMontgomery.
+
+  Section __.
+    Context (machine_wordsize : Z)
+            (n : nat)
+            (sat_limbs : nat)
+            (word_tc_mul_limbs : nat)
+            (m : Z)
+            (r' : Z)
+            (m' : Z)
+            (r'_correct : (2 ^ machine_wordsize * r') mod m = 1)
+            (m'_correct : (m * m') mod 2 ^ machine_wordsize = -1 mod 2 ^ machine_wordsize)
+            (m_small : m < (2 ^ machine_wordsize) ^ Z.of_nat n)
+            (m_big : 2 ^ machine_wordsize < m).
+
+    Notation outer_loop_body_hd := (outer_loop_body_hd machine_wordsize n sat_limbs word_tc_mul_limbs m m').
+
+    Lemma twos_complement_word_to_montgomery_no_encode_correct a
+          (Hmw : 0 < machine_wordsize)
+          (Hn : (1 < n)%nat)
+          (* (Hm : 1 < m) *)
+          (Ha : 0 <= a < 2 ^ machine_wordsize)
+      :
+        @eval machine_wordsize n (twos_complement_word_to_montgomery_no_encode machine_wordsize n m a) mod m = Z.twos_complement machine_wordsize a mod m
+        /\ valid machine_wordsize n m (twos_complement_word_to_montgomery_no_encode machine_wordsize n m a).
+    Proof.
+      unfold twos_complement_word_to_montgomery_no_encode.
+      assert (2 ^ (machine_wordsize) <= 2 ^ (machine_wordsize * Z.of_nat n)) by
+          (apply Z.pow_le_mono_r; nia).
+      assert (valid machine_wordsize n m (Partition.partition (uweight machine_wordsize) n (Z.twos_complement_opp machine_wordsize a))).
+      { unfold valid, small.
+        pose proof Z.mod_pos_bound (-a) (2^machine_wordsize) ltac:(apply Z.pow_pos_nonneg; lia).
+        split; unfold eval.
+        rewrite eval_partition, uweight_eq_alt', Z.mod_small by
+            (try rewrite twos_complement_opp_correct; try apply uwprops; nia); reflexivity.
+        rewrite eval_partition, uweight_eq_alt', twos_complement_opp_correct, Z.mod_pow_same_base_larger;
+          try apply uwprops; nia. }
+      pose proof (Hvalid := oppmod_correct machine_wordsize n m r' m' r'_correct m'_correct ltac:(lia) ltac:(lia) ltac:(lia) m_small).
+      rewrite twos_complement_neg_spec, !unfold_Let_In, select_eq with (n:=n); try (try rewrite length_partition; lia);
+        try (apply length_small with (lgr:=machine_wordsize); apply Hvalid; assumption); try apply (uweight machine_wordsize).
+
+      unfold Z.twos_complement.
+      rewrite Z.twos_complement_cond_equiv by lia.
+
+      destruct (Z.testbit a (machine_wordsize - 1)) eqn:E; cbn -[Partition.partition oppmod]; split.
+      - replace (@eval machine_wordsize n
+                  (oppmod machine_wordsize n m (Partition.partition (uweight machine_wordsize) n (Z.twos_complement_opp machine_wordsize a)))) with
+            (@eval machine_wordsize n
+              (oppmod machine_wordsize n m (Partition.partition (uweight machine_wordsize) n (Z.twos_complement_opp machine_wordsize a))) * (1 ^ n)) by (rewrite Z.pow_1_l; lia).
+
+        rewrite <- r'_correct. push_Zmod; pull_Zmod.
+        rewrite Z.pow_mul_l, Z.mul_comm, <- Z.mul_assoc, Z.mul_comm, (Z.mul_comm (r' ^ _)),  <- Zmult_mod_idemp_l,  <- eval_from_montgomerymod with (m':=m'), eval_oppmod with (r':=r'); try lia; try (try apply Hvalid; assumption).
+        push_Zmod. rewrite eval_from_montgomerymod with (r':=r'); try lia; try (try apply Hvalid; assumption).
+        push_Zmod. unfold eval; rewrite eval_partition by (apply uwprops; lia).
+        rewrite twos_complement_opp_correct. pull_Zmod.
+        rewrite uweight_eq_alt', Z.mod_pow_same_base_larger, Z.mul_opp_l, <- Z.mul_assoc, <- Z.pow_mul_l, (Z.mul_comm r'), PullPush.Z.opp_mod_mod, <- Zmult_mod_idemp_r, PullPush.Z.mod_pow_full, r'_correct, Z.pow_1_l by nia. pull_Zmod. rewrite Z.mul_1_r.
+        destruct (dec (a = 0)).
+        + subst. rewrite Z.bits_0 in *. inversion E.
+        + rewrite (Z.mod_opp_small a) by nia; apply f_equal2; [|reflexivity]; rewrite Z.mod_small; lia.
+      - apply Hvalid. assumption.
+      - unfold eval. rewrite eval_partition, uweight_eq_alt, (Z.mod_small a), (Z.mod_small a (2 ^ _)); try apply uwprops; lia.
+      - unfold valid; split.
+        + unfold small.
+          unfold eval. rewrite eval_partition, uweight_eq_alt', Z.mod_small; try (apply uwprops; lia); try nia; reflexivity.
+        + unfold eval. rewrite eval_partition, uweight_eq_alt', Z.mod_small; try (apply uwprops; lia); try nia; reflexivity.
+    Qed.
+
+    Lemma eval_twos_complement_word_to_montgomery_no_encode a
+          (Hmw : 0 < machine_wordsize)
+          (Hn : (1 < n)%nat)
+          (Hm : 1 < m)
+          (Ha : 0 <= a < 2 ^ machine_wordsize)
+      :
+        @eval machine_wordsize n (twos_complement_word_to_montgomery_no_encode machine_wordsize n m a) mod m = Z.twos_complement machine_wordsize a mod m.
+    Proof. apply twos_complement_word_to_montgomery_no_encode_correct; assumption. Qed.
+
+
+    Ltac t := repeat match goal with
+                     | |- valid _ _ _ (addmod _ _ _ _ _) => eapply addmod_correct
+                     | |- valid _ _ _ (mulmod _ _ _ _ _ _) => eapply mulmod_correct
+                     | |- valid _ _ _ (twos_complement_word_to_montgomery_no_encode _ _ _ _) => apply twos_complement_word_to_montgomery_no_encode_correct
+                     | |- valid _ _ _ _ => eassumption
+                     | |- _ => eassumption || nia
+                     end.
+
+    (** Correctness of outer loop body  *)
+    Theorem outer_loop_body_hd_correct f g v r
+            (fodd : Z.odd (tc_eval machine_wordsize sat_limbs f) = true)
+            (n1 : (1 < n)%nat)
+            (mw1 : 3 < machine_wordsize)
+            (Hf : length f = sat_limbs)
+            (Hg : length g = sat_limbs)
+
+            (sat_limbs0 : (0 < sat_limbs)%nat)
+            (word_tc_mul_limbs_eq : (word_tc_mul_limbs = 1 + sat_limbs)%nat)
+            (overflow_f : - 2 ^ (machine_wordsize * sat_limbs - 2) <
+                          tc_eval machine_wordsize sat_limbs f <
+                          2 ^ (machine_wordsize * sat_limbs - 2))
+            (overflow_g : - 2 ^ (machine_wordsize * sat_limbs - 2) <
+                          tc_eval machine_wordsize sat_limbs g <
+                          2 ^ (machine_wordsize * sat_limbs - 2))
+            (Hf2 : forall z, In z f -> 0 <= z < 2^machine_wordsize)
+            (Hg2 : forall z, In z g -> 0 <= z < 2^machine_wordsize)
+            (Hr : valid machine_wordsize n m r)
+            (Hv : valid machine_wordsize n m v) :
+      let '(f1,g1,v1,r1) := outer_loop_body_hd f g v r in
+      (tc_eval machine_wordsize sat_limbs f1,
+       tc_eval machine_wordsize sat_limbs g1,
+       @eval machine_wordsize n v1 mod m,
+       @eval machine_wordsize n r1 mod m)
+      =
+      let '(_,f1',g1',v1',r1') :=
+          hddivstep_full_iter m 1
+                            (tc_eval machine_wordsize sat_limbs f)
+                            (tc_eval machine_wordsize sat_limbs g)
+                            (@eval machine_wordsize n (from_montgomerymod machine_wordsize n m m' v) mod m)
+                            (@eval machine_wordsize n (from_montgomerymod machine_wordsize n m m' r) mod m)
+                            (Z.to_nat (machine_wordsize - 2)) in
+      (Z.twos_complement (machine_wordsize * sat_limbs) f1',
+       Z.twos_complement (machine_wordsize * sat_limbs) g1', v1', r1').
+    Proof.
+      pose proof (pow_ineq_Z2 (machine_wordsize - 1) ltac:(lia)).
+
+      assert (1 < 2 ^ machine_wordsize)
+        by (apply Zpow_facts.Zpower_gt_1; lia).
+      assert (0 < 2 ^ (machine_wordsize - 1))
+        by (apply Z.pow_pos_nonneg; lia).
+      assert (0 < 2 ^ (machine_wordsize - 2))
+        by (apply Z.pow_pos_nonneg; lia).
+      assert (2 ^ (machine_wordsize - 2) * 2 = 2 ^ (machine_wordsize - 1))
+        by (rewrite Z.mul_comm, Z.pow_mul_base by lia; apply f_equal2; lia).
+      assert (2 * (2 * (2 ^ (machine_wordsize * Z.of_nat sat_limbs - 2) * 2 ^ (machine_wordsize - 1))) = 2 ^ (machine_wordsize * (Z.of_nat (1 + sat_limbs)) - 1))
+        by (rewrite <- Zpower_exp, !Z.pow_mul_base by nia; apply f_equal2; nia).
+
+      unfold outer_loop_body_hd.
+      epose proof twos_complement_word_full_hddivstep_iter_partially_correct (machine_wordsize) 1 (nth_default 0 f 0) (nth_default 0 g 0) 1 0 0 1 (Z.to_nat (machine_wordsize - 2)) 2 _ _ _ _ _ _ _ _ _ _ _ _ _ _ _.
+
+      epose proof twos_complement_word_full_hddivsteps_partial_bounds (machine_wordsize) 1 (nth_default 0 f 0) (nth_default 0 g 0) 1 0 0 1 (Z.to_nat (machine_wordsize - 2)) 2 _ _ _ _ _ _ _ _ _ _ _ _ _.
+
+      replace (Z.of_nat (Z.to_nat (machine_wordsize - 2))) with (machine_wordsize - 2) in * by lia.
+
+      epose proof jump_hddivstep_full
+            m
+            (tc_eval machine_wordsize sat_limbs f)
+            (Z.twos_complement machine_wordsize (nth_default 0 f 0))
+            (tc_eval machine_wordsize sat_limbs g)
+            (Z.twos_complement machine_wordsize (nth_default 0 g 0))
+            (@eval machine_wordsize n (from_montgomerymod machine_wordsize n m m' v) mod m)
+            (@eval machine_wordsize n (from_montgomerymod machine_wordsize n m m' r) mod m)
+            (Z.to_nat (machine_wordsize - 2)) _ _ _ _ _ _.
+
+      rewrite Z.twos_complement_one, Z.twos_complement_zero in * by lia.
+
+      rewrite <- fold_right_fold_left_lemma with (l:=(seq 0 (Z.to_nat (machine_wordsize - 2)))) by reflexivity.
+
+      destruct (fold_left (fun (i : Z * Z * Z * Z * Z * Z * Z) (_ : nat) => twos_complement_word_full_hddivstep_aux machine_wordsize i)
+                              (seq 0 (Z.to_nat (machine_wordsize - 2))) (1, nth_default 0 f 0, nth_default 0 g 0, 1, 0, 0, 1)) as [[[[[[d1 f1] g1] u1] v1] q1] r1] eqn:E1 .
+
+      destruct (hddivstep_full_iter
+                  m 1
+                  (tc_eval machine_wordsize sat_limbs f)
+                  (tc_eval machine_wordsize sat_limbs g)
+                  (@eval machine_wordsize n (from_montgomerymod machine_wordsize n m m' v) mod m)
+                  (@eval machine_wordsize n (from_montgomerymod machine_wordsize n m m' r) mod m) (Z.to_nat (machine_wordsize - 2)))
+        as [[[[d1' f1'] g1'] v1'] r1'] eqn:E2.
+
+
+      destruct (hddivstep_spec_full'_iter
+                  1
+                  (Z.twos_complement machine_wordsize (nth_default 0 f 0))
+                  (Z.twos_complement machine_wordsize (nth_default 0 g 0))
+                  1 0 0 1 (Z.to_nat (machine_wordsize - 2)))
+        as [[[[[[d1'' f1''] g1''] u1''] v1''] q1''] r1''] eqn:E3.
+
+      rewrite !unfold_Let_In.
+
+      repeat match goal with
+             | [ |- (_, _) = (_, _) ] => apply f_equal2
+             end.
+
+      + rewrite word_tc_mul_limbs_eq in *.
+        rewrite firstn_tc_eval with (n:=(1 + sat_limbs)%nat), tc_eval_arithmetic_shiftr, tc_eval_tc_add_full;
+          repeat match goal with
+          | |- length _ = _ => autorewrite with length_distr; try lia
+          | |- context[In _] => apply arithmetic_shiftr_bounds || apply tc_add_bounds
+          | _ => assumption || lia
+          end.
+        rewrite !word_tc_mul_correct by (assumption || lia).
+        inversion H7. inversion H5.
+        replace (Z.of_nat (Z.to_nat (machine_wordsize - 2))) with (machine_wordsize - 2); lia.
+        rewrite !word_tc_mul_correct; (assumption || nia).
+      + rewrite word_tc_mul_limbs_eq in *.
+        rewrite firstn_tc_eval with (n:=(1 + sat_limbs)%nat), tc_eval_arithmetic_shiftr, tc_eval_tc_add_full;
+          repeat match goal with
+          | |- length _ = _ => autorewrite with length_distr; try lia
+          | |- context[In _] => apply arithmetic_shiftr_bounds || apply tc_add_bounds
+          | _ => assumption || lia
+          end.
+        rewrite !word_tc_mul_correct by (assumption || lia).
+        inversion H7. inversion H5.
+        replace (Z.of_nat (Z.to_nat (machine_wordsize - 2))) with (machine_wordsize - 2); lia.
+        rewrite !word_tc_mul_correct; (assumption || nia).
+      + rewrite <- (Z.mul_1_r (@eval _ _ _)), <- (Z.pow_1_l n), <- r'_correct by lia.
+        push_Zmod; pull_Zmod.
+        rewrite Z.pow_mul_l, Z.mul_comm, <- Z.mul_assoc, Z.mul_comm, (Z.mul_comm (r' ^ _)), <- Zmult_mod_idemp_l.
+        rewrite <- eval_from_montgomerymod with (m':=m'), eval_addmod with (r':=r') by t.
+        push_Zmod.
+        rewrite !eval_mulmod with (r':=r') by t.
+        push_Zmod.
+        rewrite !eval_from_montgomerymod with (r':=r') by t.
+        push_Zmod.
+        rewrite !eval_twos_complement_word_to_montgomery_no_encode by t.
+        pull_Zmod.
+        rewrite Z.mul_add_distr_r, <- !Z.mul_assoc, <- Z.pow_mul_l, (Z.mul_comm r'), !Z.mul_assoc, <- Z.mul_add_distr_r, <- Zmult_mod_idemp_r, PullPush.Z.mod_pow_full, r'_correct, Z.pow_1_l, Z.mod_1_l, Z.mul_1_r by lia.
+        inversion H7. inversion H5.
+        rewrite !eval_from_montgomerymod with (r':=r') by t.
+        push_Zmod; pull_Zmod.
+        apply f_equal2; lia.
+      + rewrite <- (Z.mul_1_r (@eval _ _ _)), <- (Z.pow_1_l n), <- r'_correct by lia.
+        push_Zmod; pull_Zmod.
+        rewrite Z.pow_mul_l, Z.mul_comm, <- Z.mul_assoc, Z.mul_comm, (Z.mul_comm (r' ^ _)), <- Zmult_mod_idemp_l.
+        rewrite <- eval_from_montgomerymod with (m':=m'), eval_addmod with (r':=r')by t.
+        push_Zmod.
+        rewrite !eval_mulmod with (r':=r')by t.
+        push_Zmod.
+        rewrite !eval_from_montgomerymod with (r':=r')by t.
+        push_Zmod.
+        rewrite !eval_twos_complement_word_to_montgomery_no_encode by t.
+        pull_Zmod.
+        rewrite Z.mul_add_distr_r, <- !Z.mul_assoc, <- Z.pow_mul_l, (Z.mul_comm r'), !Z.mul_assoc, <- Z.mul_add_distr_r, <- Zmult_mod_idemp_r, PullPush.Z.mod_pow_full, r'_correct, Z.pow_1_l, Z.mod_1_l, Z.mul_1_r by lia.
+        inversion H7. inversion H5.
+        rewrite !eval_from_montgomerymod with (r':=r') by t.
+        push_Zmod; pull_Zmod.
+        apply f_equal2; lia.
+
+        Unshelve.
+        all: lia || rewrite ?Z.twos_complement_one, ?Z.twos_complement_zero; lia || idtac.
+        rewrite eval_nth_default_0 with (m:=machine_wordsize) (n:=sat_limbs); try lia.
+        unfold tc_eval in fodd.
+        rewrite Z.twos_complement_odd in fodd.
+        rewrite Z.odd_mod2m. assumption.
+
+        lia. nia. assumption.
+        replace (Z.of_nat (Z.to_nat (machine_wordsize - 2))) with (machine_wordsize - 2) in * by lia.
+
+        lia.
+        apply Hf2.
+        destruct f. simpl in *. lia. left. reflexivity.
+        apply Hg2.
+        destruct g. simpl in *. lia. left. reflexivity.
+
+        replace (Z.of_nat (Z.to_nat (machine_wordsize - 2))) with (machine_wordsize - 2) in * by lia; lia.
+        unfold tc_eval in fodd.
+        rewrite eval_nth_default_0 with (n:=sat_limbs) (m:=machine_wordsize), Z.odd_mod2m by (assumption || lia).
+        rewrite Z.twos_complement_odd in fodd; assumption || nia.
+
+        assumption.
+        apply Z.mod_pos_bound; lia.
+        apply Z.mod_pos_bound; lia.
+
+        unfold tc_eval.
+        rewrite eval_nth_default_0 with (n:=sat_limbs) (m:=machine_wordsize), Z.twos_complement_mod, !Z.twos_complement_mod_smaller_pow; assumption || nia.
+
+        unfold tc_eval.
+        rewrite eval_nth_default_0 with (n:=sat_limbs) (m:=machine_wordsize), Z.twos_complement_mod, !Z.twos_complement_mod_smaller_pow; assumption || nia.
+    Qed.
+  End __.
+End WordByWordMontgomery.
+
+Module UnsaturatedSolinas.
+
+  Import Definitions.UnsaturatedSolinas.
+
+  Section __.
+
+    Context (limbwidth_num limbwidth_den : Z)
+            (limbwidth_good : 0 < limbwidth_den <= limbwidth_num)
+            (machine_wordsize : Z)
+            (s : Z)
+            (c : list (Z*Z))
+            (n : nat)
+            (sat_limbs : nat)
+            (word_tc_mul_limbs : nat)
+            (idxs : list nat)
+            (m_big : 2 ^ machine_wordsize < s - Associational.eval c)
+            (len_c : nat)
+            (len_idxs : nat)
+            (m_nz:s - Associational.eval c <> 0) (s_nz:s <> 0)
+            (Hn_nz : n <> 0%nat)
+            (Hc : length c = len_c)
+            (Hidxs : length idxs = len_idxs).
+
+    Notation eval := (Positional.eval (weight (limbwidth_num) (limbwidth_den)) n).
+
+    Context (balance : list Z)
+            (length_balance : length balance = n)
+            (eval_balance : eval balance mod (s - Associational.eval c) = 0).
+
+    Notation word_to_solina := (word_to_solina limbwidth_num limbwidth_den machine_wordsize s c n idxs balance).
+    Notation outer_loop_body_hd := (outer_loop_body_hd limbwidth_num limbwidth_den machine_wordsize s c n sat_limbs word_tc_mul_limbs idxs balance).
+
+    Lemma word_to_solina_length a :
+      length (word_to_solina a) = n.
+    Proof.
+      unfold word_to_solina.
+      rewrite !unfold_Let_In; rewrite length_select with (n:=n);
+        unfold carrymod, oppmod, encodemod; auto with distr_length.
+    Qed.
+
+    Hint Resolve word_to_solina_length : distr_length.
+
+    Lemma eval_word_to_solina a
+          (Hmw : 0 < machine_wordsize)
+          (Hn : (1 < n)%nat)
+          (Ha : 0 <= a < 2 ^ machine_wordsize) :
+      eval (word_to_solina a) mod (s - Associational.eval c) =
+      Z.twos_complement machine_wordsize a mod (s - Associational.eval c).
+    Proof.
+      unfold word_to_solina.
+      rewrite twos_complement_neg_spec.
+      rewrite !unfold_Let_In.
+      rewrite select_eq with (n:=n).
+
+      unfold Z.twos_complement.
+      rewrite Z.twos_complement_cond_equiv.
+
+      destruct (Z.testbit a (machine_wordsize - 1)) eqn:E. cbn -[Partition.partition oppmod].
+
+      rewrite eval_carrymod.
+      rewrite eval_oppmod.
+      push_Zmod.
+      rewrite eval_encodemod.
+      pull_Zmod.
+      rewrite twos_complement_opp_correct.
+
+      destruct (dec (a = 0)). subst. rewrite Z.bits_0 in E. inversion E.
+      pose proof Z.mod_pos_bound a (2 ^ machine_wordsize) ltac:(lia).
+      pose proof Z.mod_pos_bound (- a) (2 ^ machine_wordsize) ltac:(lia).
+
+      rewrite Z.mod_opp_small.
+      rewrite Z.mod_opp_small.
+      replace (a mod 2 ^ machine_wordsize - 2 ^ machine_wordsize) with (- (2 ^ machine_wordsize - (a mod 2 ^ machine_wordsize))) by lia.
+      rewrite Z.mod_opp_small.
+      rewrite Z.mod_small. lia. lia.
+      pose proof Z.mod_pos_bound a (2 ^ machine_wordsize) ltac:(lia). lia.  lia.
+
+      rewrite (Z.mod_opp_small a). lia. lia.
+
+      all: try lia; try assumption; unfold encodemod, oppmod; auto with distr_length.
+
+      simpl.
+      pose proof wprops limbwidth_num limbwidth_den limbwidth_good. destruct H.
+      rewrite eval_encode. rewrite (Z.mod_small _ (2 ^ _)).
+
+      reflexivity.
+      all: auto.
+
+      intros. unfold weight. apply Z.pow_nonzero. lia.
+      apply Z.opp_nonneg_nonpos.
+      apply Z.div_le_upper_bound. lia. nia. intros. specialize (weight_divides i). lia.
+
+      unfold carrymod; auto with distr_length.
+    Qed.
+
+    (** Correctness of outer loop body  *)
+    Theorem outer_loop_body_hd_correct f g v r
+            (fodd : Z.odd (tc_eval machine_wordsize sat_limbs f) = true)
+            (n1 : (1 < n)%nat)
+            (mw1 : 3 < machine_wordsize)
+            (Hf : length f = sat_limbs)
+            (Hg : length g = sat_limbs)
+            (Hv : length v = n)
+            (Hr : length r = n)
+            (sat_limbs0 : (0 < sat_limbs)%nat)
+            (word_tc_mul_limbs_eq : (word_tc_mul_limbs = 1 + sat_limbs)%nat)
+            (overflow_f : - 2 ^ (machine_wordsize * sat_limbs - 2) <
+                          tc_eval machine_wordsize sat_limbs f <
+                          2 ^ (machine_wordsize * sat_limbs - 2))
+            (overflow_g : - 2 ^ (machine_wordsize * sat_limbs - 2) <
+                          tc_eval machine_wordsize sat_limbs g <
+                          2 ^ (machine_wordsize * sat_limbs - 2))
+            (Hf2 : forall z, In z f -> 0 <= z < 2^machine_wordsize)
+            (Hg2 : forall z, In z g -> 0 <= z < 2^machine_wordsize) :
+      let '(f1,g1,v1,r1) := outer_loop_body_hd f g v r in
+      (tc_eval machine_wordsize sat_limbs f1,
+       tc_eval machine_wordsize sat_limbs g1,
+       eval v1 mod (s - Associational.eval c),
+       eval r1 mod (s - Associational.eval c))
+      =
+      let '(_,f1',g1',v1',r1') :=
+          hddivstep_full_iter (s - Associational.eval c) 1
+                            (tc_eval machine_wordsize sat_limbs f)
+                            (tc_eval machine_wordsize sat_limbs g)
+                            (eval v mod (s - Associational.eval c))
+                            (eval r mod (s - Associational.eval c))
+                            (Z.to_nat (machine_wordsize - 2)) in
+      (Z.twos_complement (machine_wordsize * sat_limbs) f1',
+       Z.twos_complement (machine_wordsize * sat_limbs) g1', v1', r1').
+    Proof.
+      pose proof (pow_ineq_Z2 (machine_wordsize - 1) ltac:(lia)).
+
+      assert (1 < 2 ^ machine_wordsize)
+        by (apply Zpow_facts.Zpower_gt_1; lia).
+      assert (0 < 2 ^ (machine_wordsize - 1))
+        by (apply Z.pow_pos_nonneg; lia).
+      assert (0 < 2 ^ (machine_wordsize - 2))
+        by (apply Z.pow_pos_nonneg; lia).
+      assert (2 ^ (machine_wordsize - 2) * 2 = 2 ^ (machine_wordsize - 1))
+        by (rewrite Z.mul_comm, Z.pow_mul_base by lia; apply f_equal2; lia).
+      assert (2 * (2 * (2 ^ (machine_wordsize * Z.of_nat sat_limbs - 2) * 2 ^ (machine_wordsize - 1))) = 2 ^ (machine_wordsize * (Z.of_nat (1 + sat_limbs)) - 1))
+        by (rewrite <- Zpower_exp, !Z.pow_mul_base by nia; apply f_equal2; nia).
+
+      unfold outer_loop_body_hd.
+      epose proof twos_complement_word_full_hddivstep_iter_partially_correct (machine_wordsize) 1 (nth_default 0 f 0) (nth_default 0 g 0) 1 0 0 1 (Z.to_nat (machine_wordsize - 2)) 2 _ _ _ _ _ _ _ _ _ _ _ _ _ _ _.
+
+      epose proof twos_complement_word_full_hddivsteps_partial_bounds (machine_wordsize) 1 (nth_default 0 f 0) (nth_default 0 g 0) 1 0 0 1 (Z.to_nat (machine_wordsize - 2)) 2 _ _ _ _ _ _ _ _ _ _ _ _ _.
+
+      replace (Z.of_nat (Z.to_nat (machine_wordsize - 2))) with (machine_wordsize - 2) in * by lia.
+
+      epose proof jump_hddivstep_full
+            (s - Associational.eval c)
+            (tc_eval machine_wordsize sat_limbs f)
+            (Z.twos_complement machine_wordsize (nth_default 0 f 0))
+            (tc_eval machine_wordsize sat_limbs g)
+            (Z.twos_complement machine_wordsize (nth_default 0 g 0))
+            (eval v mod (s - Associational.eval c))
+            (eval r mod (s - Associational.eval c))
+            (Z.to_nat (machine_wordsize - 2)) _ _ _ _ _ _.
+
+      rewrite Z.twos_complement_one, Z.twos_complement_zero in * by lia.
+
+      rewrite <- fold_right_fold_left_lemma with (l:=(seq 0 (Z.to_nat (machine_wordsize - 2)))) by reflexivity.
+
+      destruct (    fold_left (fun (i : Z * Z * Z * Z * Z * Z * Z) (_ : nat) => twos_complement_word_full_hddivstep_aux machine_wordsize i)
+                              (seq 0 (Z.to_nat (machine_wordsize - 2))) (1, nth_default 0 f 0, nth_default 0 g 0, 1, 0, 0, 1)) as [[[[[[d1 f1] g1] u1] v1] q1] r1] eqn:E1 .
+      destruct (hddivstep_full_iter
+                  (s - Associational.eval c) 1
+                  (tc_eval machine_wordsize sat_limbs f)
+                  (tc_eval machine_wordsize sat_limbs g)
+                  (eval v mod (s - Associational.eval c))
+                  (eval r mod (s - Associational.eval c))
+                  (Z.to_nat (machine_wordsize - 2)))
+        as [[[[d1' f1'] g1'] v1'] r1'] eqn:E2.
+
+      destruct (hddivstep_spec_full'_iter
+                  1
+                  (Z.twos_complement machine_wordsize (nth_default 0 f 0))
+                  (Z.twos_complement machine_wordsize (nth_default 0 g 0))
+                  1 0 0 1 (Z.to_nat (machine_wordsize - 2)))
+        as [[[[[[d1'' f1''] g1''] u1''] v1''] q1''] r1''] eqn:E3.
+
+      rewrite !unfold_Let_In.
+
+      repeat match goal with
+             | [ |- (_, _) = (_, _) ] => apply f_equal2
+             end.
+      + rewrite word_tc_mul_limbs_eq in *.
+        rewrite firstn_tc_eval with (n:=(1 + sat_limbs)%nat), tc_eval_arithmetic_shiftr, tc_eval_tc_add_full;
+          repeat match goal with
+                 | |- length _ = _ => autorewrite with length_distr; try lia
+                 | |- context[In _] => apply arithmetic_shiftr_bounds || apply tc_add_bounds
+                 | _ => assumption || lia
+                 end.
+        rewrite !word_tc_mul_correct by (assumption || lia).
+        inversion H7. inversion H5.
+        replace (Z.of_nat (Z.to_nat (machine_wordsize - 2))) with (machine_wordsize - 2); lia.
+        rewrite !word_tc_mul_correct; (assumption || nia).
+      + rewrite word_tc_mul_limbs_eq in *.
+        rewrite firstn_tc_eval with (n:=(1 + sat_limbs)%nat), tc_eval_arithmetic_shiftr, tc_eval_tc_add_full;
+          repeat match goal with
+                 | |- length _ = _ => autorewrite with length_distr; try lia
+                 | |- context[In _] => apply arithmetic_shiftr_bounds || apply tc_add_bounds
+                 | _ => assumption || lia
+                 end.
+        rewrite !word_tc_mul_correct by (assumption || lia).
+        inversion H7. inversion H5.
+        replace (Z.of_nat (Z.to_nat (machine_wordsize - 2))) with (machine_wordsize - 2); lia.
+        rewrite !word_tc_mul_correct; (assumption || nia).
+      + rewrite eval_carrymod, eval_addmod; try lia.
+        push_Zmod.
+        rewrite !eval_carry_mulmod; try lia.
+        push_Zmod.
+        rewrite !eval_word_to_solina; try lia.
+
+        inversion H7. inversion H5.
+        push_Zmod; pull_Zmod. reflexivity.
+        apply word_to_solina_length.
+        apply word_to_solina_length.
+        unfold carry_mulmod, mulmod; auto with distr_length.
+        unfold carry_mulmod, mulmod; auto with distr_length.
+        unfold addmod, carry_mulmod, mulmod; auto with distr_length.
+      + rewrite eval_carrymod, eval_addmod; try lia.
+        push_Zmod.
+        rewrite !eval_carry_mulmod; try lia.
+        push_Zmod.
+        rewrite !eval_word_to_solina; try lia.
+
+        inversion H7. inversion H5.
+        push_Zmod; pull_Zmod. reflexivity.
+        apply word_to_solina_length.
+        apply word_to_solina_length.
+        unfold carry_mulmod, mulmod; auto with distr_length.
+        unfold carry_mulmod, mulmod; auto with distr_length.
+        unfold addmod, carry_mulmod, mulmod; auto with distr_length.
+
+        Unshelve.
+        all: lia || rewrite ?Z.twos_complement_one, ?Z.twos_complement_zero; lia || idtac.
+        rewrite eval_nth_default_0 with (m:=machine_wordsize) (n:=sat_limbs); try lia.
+        unfold tc_eval in fodd.
+        rewrite Z.twos_complement_odd in fodd.
+        rewrite Z.odd_mod2m. assumption.
+
+        lia. nia. assumption.
+        replace (Z.of_nat (Z.to_nat (machine_wordsize - 2))) with (machine_wordsize - 2) in * by lia.
+
+        lia.
+        apply Hf2.
+        destruct f. simpl in *. lia. left. reflexivity.
+        apply Hg2.
+        destruct g. simpl in *. lia. left. reflexivity.
+
+        replace (Z.of_nat (Z.to_nat (machine_wordsize - 2))) with (machine_wordsize - 2) in * by lia; lia.
+        unfold tc_eval in fodd.
+        rewrite eval_nth_default_0 with (n:=sat_limbs) (m:=machine_wordsize), Z.odd_mod2m by (assumption || lia).
+        rewrite Z.twos_complement_odd in fodd; assumption || nia.
+
+        assumption.
+        apply Z.mod_pos_bound; lia.
+        apply Z.mod_pos_bound; lia.
+
+        unfold tc_eval.
+        rewrite eval_nth_default_0 with (n:=sat_limbs) (m:=machine_wordsize), Z.twos_complement_mod, !Z.twos_complement_mod_smaller_pow; assumption || nia.
+
+        unfold tc_eval.
+        rewrite eval_nth_default_0 with (n:=sat_limbs) (m:=machine_wordsize), Z.twos_complement_mod, !Z.twos_complement_mod_smaller_pow; assumption || nia.
+    Qed.
+  End __.
+
+End UnsaturatedSolinas.
