src/PushButtonSynthesis/BYInversionReificationCache.v
@@ -61,6 +61,15 @@ Module Export WordByWordMontgomery.
   Hint Rewrite (proj1 reified_outer_loop_body_gen_correct) : interp_gen_cache.
   Local Opaque reified_outer_loop_body_gen. (* needed for making [autorewrite] not take a very long time *)
 
+  Derive reified_outer_loop_body_hd_gen
+         SuchThat (is_reification_of reified_outer_loop_body_hd_gen outer_loop_body_hd)
+         As reified_outer_loop_body_hd_gen_correct.
+  Proof. Time cache_reify (). Time Qed.
+  Hint Extern 1 (_ = _) => apply_cached_reification outer_loop_body_hd (proj1 reified_outer_loop_body_hd_gen_correct) : reify_cache_gen.
+  Hint Immediate (proj2 reified_outer_loop_body_hd_gen_correct) : wf_gen_cache.
+  Hint Rewrite (proj1 reified_outer_loop_body_hd_gen_correct) : interp_gen_cache.
+  Local Opaque reified_outer_loop_body_hd_gen. (* needed for making [autorewrite] not take a very long time *)
+
   Derive reified_divstep_gen
          SuchThat (is_reification_of reified_divstep_gen divstep)
          As reified_divstep_gen_correct.
@@ -82,6 +91,15 @@ Module Export UnsaturatedSolinas.
   Hint Immediate (proj2 reified_outer_loop_body_gen_correct) : wf_gen_cache.
   Hint Rewrite (proj1 reified_outer_loop_body_gen_correct) : interp_gen_cache.
   Local Opaque reified_outer_loop_body_gen. (* needed for making [autorewrite] not take a very long time *)
+
+  Derive reified_outer_loop_body_hd_gen
+         SuchThat (is_reification_of reified_outer_loop_body_hd_gen outer_loop_body_hd)
+         As reified_outer_loop_body_hd_gen_correct.
+  Proof. Time cache_reify (). Time Qed.
+  Hint Extern 1 (_ = _) => apply_cached_reification outer_loop_body_hd (proj1 reified_outer_loop_body_hd_gen_correct) : reify_cache_gen.
+  Hint Immediate (proj2 reified_outer_loop_body_hd_gen_correct) : wf_gen_cache.
+  Hint Rewrite (proj1 reified_outer_loop_body_hd_gen_correct) : interp_gen_cache.
+  Local Opaque reified_outer_loop_body_hd_gen. (* needed for making [autorewrite] not take a very long time *)
 
   Derive reified_divstep_gen
          SuchThat (is_reification_of reified_divstep_gen divstep)
